% good luck;)
\documentclass[a4paper]{article}
\usepackage{geometry}
\geometry{left=4cm,right=4cm,top=1cm,bottom=4cm}
\title{Homework 1}
\author{Xiaoling Long\\Student ID.:81943968\\email:longxl@shanghaitech.edu.cn}
\usepackage{graphicx}
\usepackage[colorlinks,linkcolor=red]{hyperref}
\usepackage{amsmath, amsthm, amssymb}
\usepackage{subfloat}
\newtheorem{prop}{Proposition}
\usepackage{ulem}
\usepackage{indentfirst}
\begin{document}
\maketitle

\begin{description}
\item[Problem 1](4/10, \textit{A little group theory drill}):

Let $G$ be a group with group operation $*$ and identity element $e$.
Suppose that $\forall g \in G$ we have that $g * g = e$. Show that $G$
is an abelian group.
\begin{proof}We can know that,
%  \begin{equation*}
%    \forall h \in G \quad\text{s.t. } h * e=e * h
%  \end{equation*}
\begin{align*}
\forall& a,b,g \in G  \quad\intertext{We have }  a*b \in G &\ \text{and }\   g*g^{-1}=e \\
\to & \quad g =g^{-1}\\
\to & \quad a*b =(a*b)^{-1}\\
\quad&= b^{-1}*a^{-1}\\
\quad &= b*a\\
 \intertext{Finally, we get that }
 a*b&=b*a
\end{align*}
So, $G$ is an abelian group.\\
Done.
\end{proof}

\item[Problem 2](4/10, \textit{Behavior of identity element and inverses under
  group homomorphisms}):

Let $G$, $H$ be groups with group operations $*_G$, $*_H$ and identity
elements $e_G$, $e_H$ respectively. Let $\phi:G\to H$ be a group
homomorphism. Show that $\phi(e_G)=e_H$ and that $\forall g\in G$ we
have that $\phi(g^{-1})=(\phi(g))^{-1}$.
\begin{proof}
  First question.\\Because $\phi:G\to H$ is a group homomorphism.\\
  We can say that $$\forall g \in G,\exists h \in H \quad \phi(g)=h$$\\
  Then,
  \begin{align*}
    \phi(g)&=\phi(g*_G e_G)\\
    &=\phi(g)*_H \phi(e_G)\\
    &=h*_H \phi(e_G)\\
    &=h
  \end{align*}
  So we have $$h*_H\phi(e_G)=h$$
  Then,$$h^{-1}*_Hh*_H \phi(e_G)=h^{-1}*_H h$$
  $$\forall h \in H \quad h*_Hh^{-1}=h^{-1}*_Hh=e_H$$
  Finally,$$\phi(e_G)=e_H$$
  Second question.\\
  We know $$\phi(e_G)=e_H $$
   and $$\forall g \in G \quad g*g^{-1}=e_G $$
  So,
  \begin{align*}
    \phi(e_G)=\phi(g*_G g^{-1})&=\phi(g)*_H \phi(g^{-1}) \\
    &=e_H\\
  \end{align*}
  We can do $$(\phi(g))^{-1}*_H\phi(g)*_H\phi(g^{-1})=(\phi(g))^{-1}*_He_H$$
    $$\to (\phi(g))^{-1}=\phi(g^{-1})\\$$
  Done.
\end{proof}
\item[Problem 3](2/10, \textit{Group isomorphism is a transitive relation}):

Let $G$, $H$, $K$ be groups such that $G$ is isomorphic to $H$, and
$H$ is isomorphic to $K$. Show that $G$ is isomorphic to $K$.
\begin{proof}
 Show that:\\
 Let:$\phi_G,\phi_H,\psi_H,\psi_K:G\to H,H\to K , H\to G, K\to H$ \quad be group homomorsim respectively.
 \begin{align*}
   \forall g \in G \quad \exists h \in H \quad\phi_G(g)=h\\
   \forall h \in H \quad \exists k \in K \quad\phi_H(h)=k\\
   \forall k \in K \quad \exists h \in H \quad\psi_K(k)=h\\
   \forall h \in H \quad \exists g \in G \quad\psi_H(h)=g\\
   \to \forall g \in G \quad \exists k \in K \quad \phi_H(\phi_G(g))=k\\
   \&\quad \forall k \in K \quad \exists g \in G \quad \psi_H(\psi_K(k))=g
 \end{align*}
 So we can find a function $\phi$ let $$\forall g \in G \quad \exists k \in K \quad \phi(g)=k$$
 There also is a function $\psi$ let $$\forall k \in K \quad \exists g \in G \quad \psi(k)=g$$
 So, $G$ is isomorphic to $K$.\\
 Done.
\end{proof}

\end{description}
\end{document}
